src/DatalogCompilers/GridTopology.v
@@ -14,48 +14,21 @@ From coqutil Require Import Map.Interface Eqb Decidable Datatypes.List.
 From GraphSearch Require Import GraphInterface GraphImpl.
 Import ListNotations.
 
-#[global] Instance node_id_map T : map.map Node T := @SortedListList.map nat Nat.ltb SortedListNat.Nat_strict_order T.
-
-Lemma node_id_map_ok T : map.ok (node_id_map T).
-Proof. exact (@SortedListList.ok nat Nat.ltb SortedListNat.Nat_strict_order T). Qed.
-
 (* Build the grid topology graph (node set + neighbor edges) from dimensions.  Since a node id
    *is* its coordinate list, there is no destructuring/reassembly. *)
-Definition build_topo_node_set (dims : GridGraph.Dimensions) : node_id_map unit :=
+Definition build_topo_node_set (dims : GridGraph.Dimensions) : @map.rep Node unit _ :=
   List.fold_left
     (fun acc n => map.put acc n tt)
     (GridGraph.all_nodes_h dims)
     map.empty.
 
-#[global] Instance node_id_eqb : Eqb Node := list_eqb Nat.eqb.
-
-Lemma nat_eqb_dec : EqDecider Nat.eqb.
-Proof. intros x y. destruct (Nat.eqb_spec x y); constructor; assumption. Qed.
-
-#[global] Instance node_id_eqb_ok : Eqb_ok node_id_eqb.
-Proof.
-  intros a b. unfold eqb, node_id_eqb.
-  destruct (@list_eqb_spec nat Nat.eqb nat_eqb_dec a b); assumption.
-Qed.
-
-#[global] Instance node_id_graph : graph.graph Node :=
-  @GraphImpl.graph_map Node node_id_eqb node_id_eqb_ok
-    (node_id_map unit) (node_id_map_ok unit)
-    (node_id_map (node_id_map unit)) (node_id_map_ok _).
-
-#[global] Instance node_id_graph_ok : graph.ok node_id_graph.
-Proof. exact (@GraphImpl.graph_map_ok Node node_id_eqb node_id_eqb_ok
-                (node_id_map unit) (node_id_map_ok unit)
-                (node_id_map (node_id_map unit)) (node_id_map_ok _)). Qed.
-
-Definition build_topo_edges (dims : GridGraph.Dimensions) : node_id_graph :=
+Definition build_topo_edges (dims : GridGraph.Dimensions) : @graph.rep Node _ :=
   let nodes := GridGraph.all_nodes_h dims in
   List.fold_left
     (fun acc n =>
       graph.put_edges acc n (List.filter (fun n2 => GridGraph.is_neighbor dims n n2) nodes))
     nodes graph.empty.
 
-Definition make_topo_graph (dims : GridGraph.Dimensions)
-    : @ComputableGraph Node (node_id_map unit) node_id_graph :=
+Definition make_topo_graph (dims : GridGraph.Dimensions) : ComputableGraph Node :=
   {| ComputableGraph.nodes := build_topo_node_set dims;
      ComputableGraph.edges := build_topo_edges dims |}.
