src/DatalogCompilers/StringDatalog.v
@@ -8,20 +8,8 @@ From coqutil Require Import Map.Interface Map.SortedListString Eqb Decidable.
 From GraphSearch Require Import GraphInterface GraphImpl.
 Import StringDatalogParams.
 
-(* Variables and functions are strings; these are the variable-keyed maps the compiler needs. *)
-#[global] Instance var_node_set : map.map _ _ := SortedListString.map unit.
-#[global] Instance var_eqb : Eqb string_var := String.eqb.
+(* Variables and functions are strings; string-keyed sorted-list maps resolve for all of them. *)
+Existing Instance SortedListString.map.
+Existing Instance SortedListString.ok.
 
-#[global] Instance var_eqb_ok : Eqb_ok var_eqb.
-Proof. intros a b. unfold eqb, var_eqb. destruct (String.eqb_spec a b); assumption. Qed.
 
-#[global] Instance var_graph_impl : graph.graph string_var :=
-  @GraphImpl.graph_map string_var var_eqb var_eqb_ok
-    (SortedListString.map unit) (SortedListString.ok unit)
-    (SortedListString.map (SortedListString.map unit)) (SortedListString.ok _).
-
-#[global] Instance var_graph_impl_ok : graph.ok var_graph_impl :=
-  @GraphImpl.graph_map_ok string_var var_eqb var_eqb_ok
-    (SortedListString.map unit) (SortedListString.ok unit)
-    (SortedListString.map (SortedListString.map unit)) (SortedListString.ok _).
-#[global] Instance var_idx_map : map.map _ _ := SortedListString.map nat.
